bunch of coercion work

src/computational_monads/coercions.lean
@@ -10,34 +10,40 @@ This file provides a number of `has_coe` instances for different `oracle_comp` c
 The main coercions are for the append operation on `oracle_spec`,
   allowing an increase the number of oracles in a number of ways.
 This allows a computation to be written by composing computations using fewer oracles.
+
+The coercions are ordered very specifically using priority attributes,
+  to ensure that they can converge to anything in a sort of 'standard form'
+In particular, can coerce to any set of appended oracles assuming that:
+1. The target oracle list is fully left associated, which is the same associativity as `++`.
+2. The subset of original oracles in the target is in the same order.
+To match this we adopt both conventions in general, and use a standard ordering for all oracles.
+In particular we start with the basic finite oracles: `coin_oracle ++ uniform_selecting ++ ...`
 -/
 
 open oracle_comp oracle_spec distribution_semantics
 
--- TODO: α β γ
-variables (A B : Type) (spec spec' spec'' spec''' : oracle_spec)
-  (coe_spec coe_spec' coe_spec'' coe_spec''' : oracle_spec)
+variables (spec spec' spec'' spec''' : oracle_spec)
+  (coe_spec coe_spec' coe_spec'' coe_spec''' : oracle_spec) {α : Type}
 
 section uniform_select
 
 /-- coerce a coin flip into a uniform random selection of a `bool` -/
-noncomputable instance coe_coin_uniform_select :
-  has_coe (oracle_comp coin_oracle A) (oracle_comp uniform_selecting A) :=
-{ coe := λ oa, oa.simulate' ⟪λ _ _, $ᵗ bool⟫ () }
+noncomputable instance coe_coin_uniform_select (α) :
+  has_coe (oracle_comp coin_oracle α) (oracle_comp uniform_selecting α) :=
+{ coe := λ oa, oa.default_simulate' ⟪λ _ _, $ᵗ bool⟫ }
 
 noncomputable example : oracle_comp uniform_selecting bool :=
 do {b ← coin, b' ←$ᵗ bool, return (band b b')}
 
-lemma coe_coin_uniform_select_def (oa : oracle_comp coin_oracle A) :
-  (↑oa : oracle_comp uniform_selecting A) = oa.simulate' ⟪λ _ _, $ᵗ bool⟫ () := rfl
+lemma coe_coin_uniform_select_def (oa : oracle_comp coin_oracle α) :
+  (↑oa : oracle_comp uniform_selecting α) = oa.default_simulate' ⟪λ _ _, $ᵗ bool⟫ := rfl
 
 /-- Coercing to a `uniform_selecting` oracle doesn't change the underlying distribution -/
 @[simp]
-lemma coe_coin_uniform_select_equiv_coin :
-  Π {A : Type} (oc : oracle_comp coin_oracle A),
-    (↑oc : oracle_comp uniform_selecting A) ≃ₚ oc
-| _ (pure' A a) := by simp [coe_coin_uniform_select_def, pmf.pure_map]
-| _ (bind' A B oa ob) := begin
+lemma coe_coin_uniform_select_equiv_coin : Π {α : Type} (oc : oracle_comp coin_oracle α),
+    (↑oc : oracle_comp uniform_selecting α) ≃ₚ oc
+| _ (pure' α a) := by simp [coe_coin_uniform_select_def, pmf.pure_map]
+| _ (bind' α β oa ob) := begin
   rw [coe_coin_uniform_select_def],
   refine (stateless_oracle.simulate'_query_equiv_of_equiv _ _ _ _),
   intros i t,
@@ -53,158 +59,167 @@ end uniform_select
 
 section coe_append
 
+section coe_append_right
+
 /-- Coerce a computation to one with access to another oracle on the right,
   forwarding the old queries to the left side of the combined set of oracles -/
-instance coe_append_right :
-  has_coe (oracle_comp spec A) (oracle_comp (spec ++ spec') A) :=
-{ coe := default_simulate' ⟪λ i t, let i' : (spec ++ spec').ι := sum.inl i in query i' t⟫ }
+@[priority std.priority.default-10]
+instance coe_append_right (α) : has_coe (oracle_comp spec α) (oracle_comp (spec ++ spec') α) :=
+{ coe := default_simulate' ⟪λ i, let i' : (spec ++ spec').ι := sum.inl i in query i'⟫ }
 
 -- TODO: other versions of this
-lemma coe_append_right_def (oa : oracle_comp spec A) : (↑oa : oracle_comp (spec ++ spec') A) =
+lemma coe_append_right_def (oa : oracle_comp spec α) : (↑oa : oracle_comp (spec ++ spec') α) =
   oa.default_simulate' ⟪λ i t, let i' : (spec ++ spec').ι := sum.inl i in query i' t⟫ := rfl
 
-lemma coe_append_right_pure_equiv [spec.finite_range] [spec'.finite_range] (a : A) :
-  (↑(pure a : oracle_comp spec A) : oracle_comp (spec ++ spec') A)
-    ≃ₚ (pure a : oracle_comp (spec ++ spec') A) :=
+section distribution_semantics
+
+lemma coe_append_right_pure_equiv [spec.finite_range] [spec'.finite_range] (a : α) :
+  (↑(pure a : oracle_comp spec α) : oracle_comp (spec ++ spec') α)
+    ≃ₚ (pure a : oracle_comp (spec ++ spec') α) :=
 default_simulate'_pure_equiv _ a
 
-lemma simulate_coe_append_right_equiv [spec''.finite_range] (oa : oracle_comp spec A)
+/-- The right hand simulation oracle is irrelevent to simulate an append right coercion -/
+lemma simulate'_coe_append_right_equiv [spec.finite_range] [spec'.finite_range]
+  [spec''.finite_range] (oa : oracle_comp spec α) (so : simulation_oracle spec spec'')
+  (so' : simulation_oracle spec' spec'') (s : so.S × so'.S) :
+  simulate' (so ++ₛ so') ↑oa s ≃ₚ simulate' so oa s.1 :=
+begin
+  induction oa with α a α β oa ob i t,
+  { rw [pure'_eq_pure, simulate'_pure, map_pure_equiv, simulate'_equiv_of_equiv _ _
+      (coe_append_right_pure_equiv spec spec' a), simulate'_pure_equiv] },
+  { sorry },
+  { sorry }
+end
+
+lemma simulate_coe_append_right_equiv [spec''.finite_range] (oa : oracle_comp spec α)
   (so : simulation_oracle spec spec'') (so' : simulation_oracle spec' spec'') (s : so.S × so'.S) :
   simulate (so ++ₛ so') ↑oa s ≃ₚ do { ⟨a, s'⟩ ← simulate so oa s.1, pure (a, s', s.2) } :=
 sorry
 
-lemma simulate'_coe_append_right_equiv [spec.finite_range] [spec'.finite_range] [spec''.finite_range]
-  (oa : oracle_comp spec A)
-  (so : simulation_oracle spec spec'') (so' : simulation_oracle spec' spec'') (s : so.S × so'.S) :
-  simulate' (so ++ₛ so') ↑oa s ≃ₚ simulate' so oa s.1 :=
-begin
-  induction oa with A a A B oa ob i t,
-  {
-    
-    simp only [pure'_eq_pure, simulate'_pure, map_pure_equiv, eval_distribution_return],
-    refine trans (simulate'_map_equiv _ _ _ _) _,
-    rw [simulate_pure, simulate'_pure, map_map_pure_equiv],
-    refl,
-  },
-  {
-    sorry,
-  },
-  {
-    sorry,
-  }
-end
+end distribution_semantics
 
--- lemma simulate_coe_append_right (oa : oracle_comp spec A) (so : simulation_oracle spec spec')
---   (s : so.S × unit) :
---   (simulate' (so +++ₛ (identity_oracle spec'')) (↑oa : oracle_comp (spec ++ spec'') A) s) =
---     ↑(simulate' so oa s.1) :=
--- sorry
+end coe_append_right
 
-instance coe_append_left :
-  has_coe (oracle_comp spec A) (oracle_comp (spec' ++ spec) A) :=
-{ coe := λ oc, oc.simulate'
-    ⟪ (λ i t, let i' : (spec' ++ spec).ι := sum.inr i in query i' t) ⟫ () }
+section coe_append_left
 
-instance coe_right_side_append [∀ A, has_coe (oracle_comp coe_spec A) (oracle_comp coe_spec' A)] :
-  has_coe (oracle_comp (spec ++ coe_spec) A) (oracle_comp (spec ++ coe_spec') A) :=
-{ coe := λ oc, oc.simulate' ⟪λ i, sum.rec
-    (λ i' t, (query i' t : oracle_comp (spec ++ coe_spec') (spec.range i')))
-    (λ i' t, (query i' t : oracle_comp (spec ++ coe_spec') (coe_spec.range i')))
-  i⟫ () }
+/-- Coerce a computation to one with access to another oracle on the left,
+  forwarding the old queries to the left side of the combined set of oracles -/
+@[priority std.priority.default-10]
+instance coe_append_left (α) : has_coe (oracle_comp spec α) (oracle_comp (spec' ++ spec) α) :=
+{ coe := default_simulate' ⟪λ i, let i' : (spec' ++ spec).ι := sum.inr i in query i'⟫ }
 
-instance coe_left_side_append [∀ A, has_coe (oracle_comp coe_spec A) (oracle_comp coe_spec' A)] :
-  has_coe (oracle_comp (coe_spec ++ spec) A) (oracle_comp (coe_spec' ++ spec) A) :=
-{ coe := λ oc, oc.simulate' ⟪λ i, sum.rec
-    (λ i' t, (query i' t : oracle_comp (coe_spec' ++ spec) (coe_spec.range i')))
-    (λ i' t, (query i' t : oracle_comp (coe_spec' ++ spec) (spec.range i')))
-  i⟫ () }
+end coe_append_left
 
-instance coe_both_sides_append [∀ A, has_coe (oracle_comp coe_spec A) (oracle_comp coe_spec' A)]
-  [∀ A, has_coe (oracle_comp coe_spec'' A) (oracle_comp coe_spec''' A)] :
-  has_coe (oracle_comp (coe_spec ++ coe_spec'') A) (oracle_comp (coe_spec' ++ coe_spec''') A) :=
-{ coe := λ oc, oc.simulate' ⟪λ i, sum.rec
-    (λ i' t, (query i' t : oracle_comp (coe_spec' ++ coe_spec''') (coe_spec.range i')))
-    (λ i' t, (query i' t : oracle_comp (coe_spec' ++ coe_spec''') (coe_spec''.range i')))
-  i⟫ () }
 
-instance coe_append_right_of_coe [has_coe (oracle_comp coe_spec A) (oracle_comp coe_spec' A)] :
-  has_coe (oracle_comp coe_spec A) (oracle_comp (coe_spec' ++ spec'') A) :=
-{ coe := coe }
 
-instance coe_append_left_of_coe [has_coe (oracle_comp coe_spec A) (oracle_comp coe_spec' A)] :
-  has_coe (oracle_comp coe_spec A) (oracle_comp (spec'' ++ coe_spec') A) :=
-{ coe := coe }
+instance coe_append_right_of_coe (α) [has_coe (oracle_comp coe_spec α) (oracle_comp coe_spec' α)] :
+  has_coe (oracle_comp coe_spec α) (oracle_comp (coe_spec' ++ spec) α) :=
+{ coe := λ oa, ↑oa }
 
-@[priority 1001]
-instance coe_append_assoc :
-  has_coe (oracle_comp (spec ++ (spec' ++ spec'')) A) (oracle_comp (spec ++ spec' ++ spec'') A) :=
+-- instance coe_append_left_of_coe [has_coe (oracle_comp coe_spec α) (oracle_comp coe_spec' α)] :
+--   has_coe (oracle_comp coe_spec α) (oracle_comp (spec'' ++ coe_spec') α) :=
+-- { coe := coe }
+
+
+
+section coe_right_side_append
+
+/-- Coerce the oracle on the right side of an existing set of appended oracles -/
+@[priority std.priority.default+5]
+instance coe_right_side_append (α) [∀ α, has_coe (oracle_comp coe_spec α) (oracle_comp coe_spec' α)] :
+  has_coe (oracle_comp (spec ++ coe_spec) α) (oracle_comp (spec ++ coe_spec') α) :=
+{ coe := λ oc, oc.default_simulate' ⟪λ i, match i with
+  | (sum.inl i') := (λ t, (query i' t : oracle_comp (spec ++ coe_spec') (spec.range i')))
+  | (sum.inr i') := (λ t, (query i' t : oracle_comp (spec ++ coe_spec') (coe_spec.range i')))
+end ⟫ }
+
+end coe_right_side_append
+
+section coe_left_side_append
+
+/-- Coerce the oracle on the left side of an existing set of appended oracles -/
+@[priority std.priority.default+5]
+instance coe_left_side_append (α) [∀ α, has_coe (oracle_comp coe_spec α) (oracle_comp coe_spec' α)] :
+  has_coe (oracle_comp (coe_spec ++ spec) α) (oracle_comp (coe_spec' ++ spec) α) :=
+{ coe := λ oc, oc.simulate' ⟪λ i, match i with
+| (sum.inl i') := (λ t, (query i' t : oracle_comp (coe_spec' ++ spec) (coe_spec.range i')))
+| (sum.inr i') := (λ t, (query i' t : oracle_comp (coe_spec' ++ spec) (spec.range i')))
+end⟫ () }
+
+end coe_left_side_append
+
+section coe_append_assoc
+
+/-- Coerce towards a standardized append ordering (matching the `infixl` declaration for `++`) -/
+@[priority std.priority.default+10]
+instance coe_append_assoc (α) :
+  has_coe (oracle_comp (spec ++ (spec' ++ spec'')) α) (oracle_comp (spec ++ spec' ++ spec'') α) :=
 ⟨λ oc, oc.simulate' ⟪λ i, match i with 
-| (sum.inl i) :=
-    λ t, let i' : (spec ++ spec' ++ spec'').ι := sum.inl (sum.inl i) in query i' t
-| (sum.inr (sum.inl i)) :=
-    λ t, let i' : (spec ++ spec' ++ spec'').ι := sum.inl (sum.inr i) in query i' t
-| (sum.inr (sum.inr i)) := 
-    λ t, let i' : (spec ++ spec' ++ spec'').ι := sum.inr i in query i' t
+| (sum.inl i) := let i' : (spec ++ spec' ++ spec'').ι := sum.inl (sum.inl i) in query i'
+| (sum.inr (sum.inl i)) := let i' : (spec ++ spec' ++ spec'').ι := sum.inl (sum.inr i) in query i'
+| (sum.inr (sum.inr i)) := let i' : (spec ++ spec' ++ spec'').ι := sum.inr i in query i'
 end⟫ ()⟩
+
+end coe_append_assoc
 
 section examples
 
 -- This set of examples serves as sort of a "unit test" for the coercions above
-variable [h : ∀ A, has_coe (oracle_comp coe_spec A) (oracle_comp coe_spec' A)]
+variable [h : ∀ α, has_coe (oracle_comp coe_spec α) (oracle_comp coe_spec' α)]
 include h
 
 -- coerce a single `coin_oracle` and then append extra oracles
-example (oa : oracle_comp coe_spec A) :
-  oracle_comp (coe_spec' ++ spec' ++ spec'') A := ↑oa
-example (oa : oracle_comp coe_spec A) :
-  oracle_comp (spec ++ coe_spec' ++ spec') A := ↑oa
-example (oa : oracle_comp coe_spec A) :
-  oracle_comp (spec ++ spec' ++ coe_spec') A := ↑oa
+example (oa : oracle_comp coe_spec α) :
+  oracle_comp (coe_spec' ++ spec' ++ spec'') α := ↑oa
+example (oa : oracle_comp coe_spec α) :
+  oracle_comp (spec ++ coe_spec' ++ spec') α := ↑oa
+example (oa : oracle_comp coe_spec α) :
+  oracle_comp (spec ++ spec' ++ coe_spec') α := ↑oa
 
 -- coerce left side of append and then append on additional oracles
-example (oa : oracle_comp (coe_spec ++ spec) A) :
-  oracle_comp (coe_spec' ++ spec ++ spec') A := ↑oa
-example (oa : oracle_comp (coe_spec ++ spec) A) :
-  oracle_comp (coe_spec' ++ spec' ++ spec) A := ↑oa
-example (oa : oracle_comp (coe_spec ++ spec) A) :
-  oracle_comp (spec' ++ coe_spec' ++ spec) A := ↑oa
+example (oa : oracle_comp (coe_spec ++ spec) α) :
+  oracle_comp (coe_spec' ++ spec ++ spec') α := ↑oa
+example (oa : oracle_comp (coe_spec ++ spec) α) :
+  oracle_comp (coe_spec' ++ spec' ++ spec) α := ↑oa
+example (oa : oracle_comp (coe_spec ++ spec) α) :
+  oracle_comp (spec' ++ coe_spec' ++ spec) α := ↑oa
 
 -- coerce right side of append and then append on additional oracles
-example (oa : oracle_comp (spec ++ coe_spec) A) :
-  oracle_comp (spec ++ coe_spec' ++ spec') A := ↑oa
-example (oa : oracle_comp (spec ++ coe_spec) A) :
-  oracle_comp (spec ++ spec' ++ coe_spec') A := ↑oa
-example (oa : oracle_comp (spec ++ coe_spec) A) :
-  oracle_comp (spec' ++ spec ++ coe_spec') A := ↑oa
+example (oa : oracle_comp (spec ++ coe_spec) α) :
+  oracle_comp (spec ++ coe_spec' ++ spec') α := ↑oa
+example (oa : oracle_comp (spec ++ coe_spec) α) :
+  oracle_comp (spec ++ spec' ++ coe_spec') α := ↑oa
+example (oa : oracle_comp (spec ++ coe_spec) α) :
+  oracle_comp (spec' ++ spec ++ coe_spec') α := ↑oa
 
 -- coerce an inside part while also applying associativity
-example (oa : oracle_comp (spec ++ (spec' ++ coe_spec)) A) :
-  oracle_comp (spec ++ spec' ++ coe_spec') A := ↑oa
-example (oa : oracle_comp (spec ++ (coe_spec ++ spec')) A) :
-  oracle_comp (spec ++ coe_spec' ++ spec') A := ↑oa
-example (oa : oracle_comp (coe_spec ++ (spec ++ spec')) A) :
-  oracle_comp (coe_spec' ++ spec ++ spec') A := ↑oa
-
-end examples
-
-end coe_append
+example (oa : oracle_comp (spec ++ (spec' ++ coe_spec)) α) :
+  oracle_comp (spec ++ spec' ++ coe_spec') α := ↑oa
+example (oa : oracle_comp (spec ++ (coe_spec ++ spec')) α) :
+  oracle_comp (spec ++ coe_spec' ++ spec') α := ↑oa
+example (oa : oracle_comp (coe_spec ++ (spec ++ spec')) α) :
+  oracle_comp (coe_spec' ++ spec ++ spec') α := ↑oa
 
 /-- coercion makes it possible to mix computations on individual oracles -/
 noncomputable example {spec : oracle_spec} : oracle_comp (uniform_selecting ++ spec) bool := 
 do { n ←$[0..10], if n ≤ 3 then return ff else coin }
+
+end examples
+
+end coe_append
 
 section coe_simulation_oracle
 
 /-- Use a coercion on the resulting type of a simulation to coerce the simulation oracle itself.
   This allows for greater flexibility when specifying the simulation oracle when
     both the initial and final `oracle_spec` are some appended set of oracles -/
-instance {spec spec' spec'' : oracle_spec}
-  [∀ α, has_coe (oracle_comp spec' α) (oracle_comp spec'' α)] :
-  has_coe (simulation_oracle spec spec') (simulation_oracle spec spec'') :=
+instance [∀ α, has_coe (oracle_comp coe_spec α) (oracle_comp coe_spec' α)] :
+  has_coe (simulation_oracle spec coe_spec) (simulation_oracle spec coe_spec') :=
 { coe := λ so, { S := so.S, default_state := so.default_state, o := λ i x, ↑(so.o i x) } }
 
-example (so : simulation_oracle spec spec') :
-  simulation_oracle spec (spec ++ spec' ++ spec'') := ↑so
+/-- Coerce a simulation oracle to include an additional number of resulting oracles -/
+example (so : simulation_oracle coe_spec coe_spec') :
+  simulation_oracle coe_spec (coe_spec' ++ spec ++ spec') := ↑so
 
 /-- Can use coercions to seperately simulate both sides of appended oracle specs -/
 example (so : simulation_oracle spec spec'') (so' : simulation_oracle spec' spec''') :
